Added missing file [base_logic_extension].

coq-osiris/theories/adequacy/ewp_adequacy.v
@@ -2,29 +2,273 @@ From iris.proofmode Require Import base tactics classes.
 From iris.base_logic.lib Require Import iprop wsat gen_heap.
 From iris.program_logic Require Import weakestpre adequacy.
 
-From osiris.program_logic Require Import ewp basic_rules tactics.
+From osiris.program_logic Require Import wp_step ewp basic_rules tactics.
+From osiris.adequacy.satisfiable Require Import satisfiable.
 
+Definition WPTP `{!osirisGS Σ} (t : list (thread * micro val exn)) Φs : iProp Σ :=
+  ([∗ list] '(ι, e);Φ ∈ t;Φs, EWP e @ ⊤ <| (ι, ⊥) |> {{ Φ }}).
 
-(* -------------------------------------------------------------------------- *)
-Section ewp_wp.
+Lemma wp_wptp `{!osirisGS Σ} ι e Φ:
+  EWP e @ ⊤ <| (ι, ⊥) |> {{ Φ }} ⊢ WPTP [(ι, e)] [Φ].
+Proof. by rewrite /WPTP big_sepL2_singleton. Qed.
 
-  Import ewp_rules_tactics.
+(* Compositional Lemmas for Adequacy *)
+Section satisfiability_weakest_pre.
+  Context `{!osirisGS Σ}.
 
-  (*  We show an adequacy of a closed program using the fact that the adequacy of
-    [EWP] is a consequence of the adequacy of [WP]. This is following the adequacy
-    proof of [Hazel] (de Vilhena & Pottier) *)
-
-  Lemma ewp_imp_wp {Σ}
-    {osiris : osirisGS Σ}
-    E ι (m : micro val exn) (Φ : outcome2 val exn -> _) :
-    EWP m @ E <| (ι, ⊥) |> {{ Φ }} -∗ WP m @ NotStuck; E {{ Φ }} : iProp Σ.
+  Lemma wp_step {A X} m F E ι Ψ (e1 : micro A X) σ1 π1 e2 σ2 π2 efs Φ :
+    wp_step.wp_step (σ1, π1, e1, ι) (σ2, π2, e2, efs) →
+    SAT m F []
+      (state_interp (σ1, π1) ∗ EWP e1 @ E <| (ι, Ψ) |> {{ Φ }}) →
+    SAT m F []
+      (state_interp (σ2, π2) ∗ EWP e2 @ E <| (ι, Ψ) |> {{ Φ }} ∗ ([∗ list] '(ι', e) ∈ efs, EWP e @ ⊤ <| (ι', ⊥) |> {{ λ _, True }})).
   Proof.
-  Abort.
+    intros Hstep Hsat. eapply SAT_mono in Hsat. eapply SAT_mono in Hsat; last first.
+    { iIntros "[HSI Hwp]". rewrite ewp_unfold /ewp_pre.
+      rewrite (wp_step_is_EStep _ _ _ _ _ _ _ _ Hstep).
+      iSpecialize ("Hwp" with "HSI").
 
-  (* This strategy no longer works, because the Iris-instantiate [WP] is not
-     able to step through forks or joins. *)
+      ewp_case e1.
+      rewrite (val_stuck e1 σ1 κ e2 σ2 efs) //.
+      iSpecialize ("Hwp" $! σ1 ns κ κs nt with "HSI").
+      iExact "Hwp". }
+    eapply SAT_fupd in Hsat.
+    eapply SAT_mono in Hsat; last first.
+    { iIntros "[_ Hwp]". iSpecialize ("Hwp" $! e2 σ2 efs Hstep). iExact "Hwp". }
+    eapply (SAT_frame_resource _ (view ∅)) in Hsat; last apply _.
+    eapply SAT_later_credits_credit_wand in Hsat.
+    eapply SAT_unframe_resource in Hsat.
+    eapply SAT_elim_iterated in Hsat; last first.
+    { intros Q Hsat'. eapply SAT_fupd, SAT_later, SAT_fupd, Hsat'. }
+    eapply SAT_fupd in Hsat. eexists _. eapply Hsat.
+  Qed.
 
-End ewp_wp.
+  Lemma wp_not_stuck m F E e σ Φ ns nt κs n:
+    SAT m F [view E; supply n] (state_interp σ ns κs nt ∗ WP e @ NotStuck; E {{ Φ }}) →
+    not_stuck e σ.
+  Proof.
+    intros Hsat. rewrite /not_stuck. destruct (to_val e) eqn: He; first by eauto.
+    right. eapply SAT_mono with (Q := (|={E, ∅}=> ⌜reducible e σ⌝)%I) in Hsat.
+    { eapply SAT_fupd in Hsat. by eapply SAT_elim in Hsat. }
+    iIntros "[SI Hwp]". rewrite wp_unfold /wp_pre.
+    rewrite He. iMod ("Hwp" $! σ ns [] κs nt with "SI") as "[$ _]".
+    by iModIntro.
+  Qed.
+
+  Lemma wp_postcondition m F E s e Φ v n:
+    SAT m F [view E; supply n] (WP e @ s; E {{ Φ }}) →
+    to_val e = Some v →
+    SAT m F [view E; supply n] (Φ v).
+  Proof.
+    intros Hsat Hval. eapply SAT_mono in Hsat; last first.
+    { iIntros "Hwp". rewrite wp_unfold /wp_pre Hval. iExact "Hwp". }
+    by eapply SAT_fupd in Hsat.
+  Qed.
+
+
+
+  Lemma wptp_length m F s Rs es Φs :
+    SAT m F Rs (WPTP s es Φs) → length es = length Φs.
+  Proof.
+    intros Hsat. eapply SAT_elim, SAT_mono, Hsat. rewrite /WPTP. by iApply big_sepL2_length.
+  Qed.
+
+  Lemma wptp_extract_wp m F Rs s es1 e es2 Φs :
+    SAT m F Rs (WPTP s (es1 ++ e :: es2) Φs) →
+    ∃ Φ1s Φ2s Φ, Φs = Φ1s ++ Φ :: Φ2s ∧ length Φ1s = length es1 ∧ length Φ2s = length es2 ∧
+      SAT m F Rs (WP e @ s; ⊤ {{ Φ }} ∗ WPTP s (es1 ++ es2) (Φ1s ++ Φ2s)).
+  Proof.
+    intros Hsat. eapply wptp_length in Hsat as Hlen. symmetry in Hlen.
+    specialize (lookup_lt_is_Some_2 Φs (length es1)) as [Φ Hrest].
+    { rewrite Hlen app_length /=. lia. }
+    eapply take_drop_middle in Hrest as Hsplit.
+    eexists _, _, _. split_and!; first done.
+    - rewrite take_length Hlen app_length /=. lia.
+    - rewrite drop_length Hlen app_length /=. lia.
+    - eapply SAT_mono, Hsat. rewrite -{1}Hsplit.
+      rewrite /WPTP. iIntros "Hx". iDestruct (big_sepL2_app_inv with "Hx") as "[$ Hx2]".
+      { rewrite take_length Hlen app_length /=. lia. }
+      iDestruct "Hx2" as "[$ $]".
+  Qed.
+
+  Lemma wptp_step m F n s es1 es2 σ1 σ2 κ κs Φs ns nt :
+    SAT m F [view ⊤; supply n] (state_interp σ1 ns (κ ++ κs) nt ∗ WPTP s es1 Φs) →
+    step (es1,σ1) κ (es2, σ2) →
+    ∃ n' nt', SAT m F [view ⊤; supply n'] (state_interp σ2 (S ns) κs (nt + nt') ∗ WPTP s es2 (Φs ++ replicate nt' fork_post)).
+  Proof.
+    intros Hsat Hstep. destruct Hstep as [e1' σ1' e2' σ2' efs t2' t3 Hstep]; simplify_eq/=.
+    rewrite -SAT_frame_cons in Hsat.
+    eapply wptp_extract_wp in Hsat as (Φ1s & Φ2s & Φ & -> & Hlen1 & Hlen2 & Hsat).
+    rewrite SAT_frame_cons in Hsat.
+    eapply SAT_mono in Hsat; last first.
+    { iIntros "(SI & Hwp & Hwps)". iCombine "Hwps SI Hwp" as "Hx". iExact "Hx". }
+    rewrite -SAT_frame_cons in Hsat.
+    eapply wp_step in Hsat as (n' & Hsat); last done.
+    rewrite SAT_frame_cons in Hsat.
+    eexists _, _. eapply SAT_mono, Hsat.
+    iIntros "(Hwps & SI & Hwp & Hforks)". rewrite Nat.add_comm. iFrame "SI".
+    iDestruct (big_sepL2_app_inv with "Hwps") as "[Hwps1 Hwps2]"; first auto.
+    rewrite -app_assoc /=. rewrite /WPTP. iFrame.
+    rewrite big_sepL2_replicate_r //.
+  Qed.
+
+  Lemma wptp_steps m F n k s es1 es2 σ1 σ2 κs κs' Φs ns nt :
+    SAT m F [view ⊤; supply n] (state_interp σ1 ns (κs ++ κs') nt ∗ WPTP s es1 Φs) →
+    language.nsteps k (es1, σ1) κs (es2, σ2) →
+    ∃ n' nt', SAT m F [view ⊤; supply n'] (state_interp σ2 (ns + k) κs' (nt + nt') ∗ WPTP s es2 (Φs ++ replicate nt' fork_post)).
+  Proof.
+    induction k as [|k IH] in  n, es1, σ1, ns, κs, nt, Φs |-*; intros Hsat Hsteps.
+    - revert Hsat. inversion_clear Hsteps. exists n, 0. rewrite !right_id !Nat.add_0_r //.
+    - revert Hsat. inversion_clear Hsteps as [|?? [t1' σ1']]. rewrite -app_assoc. intros Hsat.
+      eapply wptp_step in Hsat as (n' & nt' & Hsat); last done.
+      eapply IH in Hsat as (n'' & nt'' & Hsat); last done.
+      exists n'', (nt' + nt''). rewrite !Nat.add_assoc.
+      revert Hsat. rewrite -app_assoc replicate_add //= Nat.add_succ_r //.
+  Qed.
+
+  Lemma wptp_not_stuck m F n e es σ ns κs nt Φs:
+    SAT m F [view ⊤; supply n] (state_interp σ ns κs nt ∗ WPTP NotStuck es Φs) →
+    e ∈ es →
+    not_stuck e σ.
+  Proof.
+    intros Hsat [i Hlook]%elem_of_list_lookup_1.
+    eapply take_drop_middle in Hlook as Hsplit.
+    rewrite -Hsplit in Hsat. rewrite -SAT_frame_cons in Hsat.
+    eapply wptp_extract_wp in Hsat as (Φ1s & Φ2s & Φ & -> & Hlen1 & Hlen2 & Hsat).
+    rewrite SAT_frame_cons in Hsat.
+    eapply SAT_mono in Hsat; last first.
+    { iIntros "(SI & Hwp & Hwps)". iCombine "Hwps SI Hwp" as "Hx". iExact "Hx". }
+    rewrite -SAT_frame_cons in Hsat.
+    by eapply wp_not_stuck in Hsat.
+  Qed.
+
+
+  Lemma wptp_postconditions m F n s es Φs:
+    SAT m F [view ⊤; supply n] (WPTP s es Φs) →
+    SAT m F [view ⊤; supply n] ([∗ list] e;Φ ∈ es; Φs, from_option Φ (WP e @ s; ⊤ {{ Φ }}) (to_val e)).
+  Proof.
+    induction es as [|e es IH] in Φs, F |-*; intros Hsat.
+    - eapply wptp_length in Hsat as Hlen. destruct Φs; last done. eapply Hsat.
+    - eapply wptp_length in Hsat as Hlen. destruct Φs as [|Φ Φs]; first done.
+      revert Hsat. rewrite /WPTP /=. intros Hsat.
+      rewrite -SAT_frame_cons. eapply IH. rewrite SAT_frame_cons.
+      rewrite bi.sep_comm. revert Hsat. rewrite bi.sep_comm.
+      rewrite -!SAT_frame_cons. destruct (to_val e) eqn:Heq.
+      + intros Hsat. eapply SAT_mono, wp_postcondition; eauto.
+      + eapply SAT_mono. by iIntros "$".
+  Qed.
+
+
+  (* composing the adequacy lemmas *)
+  Lemma wptp_adequacy m F n k s es1 es2 nt ns κs κs' σ1 σ2 Φs:
+    SAT m F [view ⊤; supply n] (state_interp σ1 ns (κs ++ κs') nt ∗ WPTP s es1 Φs) →
+    language.nsteps k (es1, σ1) κs (es2, σ2) →
+    ∃ n' nt', SAT m F [view ⊤; supply n']
+      (state_interp σ2 (ns + k) κs' (nt + nt') ∗ ([∗ list] e;Φ ∈ es2; (Φs ++ replicate nt' fork_post), from_option Φ (WP e @ s; ⊤ {{ Φ }}) (to_val e)))
+    ∧ (∀ e, s = NotStuck → e ∈ es2 → not_stuck e σ2).
+  Proof.
+    intros Hsat Hsteps. eapply wptp_steps in Hsat as (n' & nt' & Hsat); last done.
+    eexists _, _. split.
+    - rewrite -SAT_frame_cons in Hsat. eapply wptp_postconditions in Hsat.
+      rewrite SAT_frame_cons in Hsat. eauto using wptp_not_stuck.
+    - intros e -> Hel. eapply wptp_not_stuck; eauto.
+  Qed.
+
+
+  Lemma wp_adequacy m F n κs s e es σ1 σ2 φ nt ns k :
+    (* if we can prove satisfiable of a weakest pre and the state interpretation *)
+    SAT m F [view ⊤; supply n] (state_interp σ1 nt κs ns ∗ WP e @ s; ⊤ {{ v, ⌜φ v⌝%I }}) →
+    (* and we take a k-step execution to [e'] and some forked of threads *)
+    language.nsteps k ([e], σ1) κs (es, σ2) →
+    (* then no thread is stuck and if the main thread terminates in a value, it satisfies the postcondition *)
+    (∀ v es', es = language.of_val v :: es' → φ v) ∧
+    (∀ e, s = NotStuck → e ∈ es → not_stuck e σ2).
+  Proof.
+    intros Hsat Hsteps. rewrite wp_wptp in Hsat.
+    replace κs with (κs ++ []) in Hsat by rewrite app_nil_r //.
+    eapply wptp_adequacy in Hsat as (n' & nt' & Hsat); eauto.
+    destruct Hsat as (Hsat & Hnstuck). split; last eapply Hnstuck.
+    intros v es' ->; simpl in *. rewrite to_of_val /= in Hsat.
+    eapply SAT_elim, SAT_mono, Hsat. iIntros "(_ & $ & _)".
+  Qed.
+
+End satisfiability_weakest_pre.
+
+
+
+(* Lemma for handling the allocation of invariants and later credits. *)
+(* To use it, you should:
+    - pick a type X that carries all of the global ghost names for your language (e.g., [heapGS] for HeapLang)
+    - pick a function [I] that takes the ghost names and produces an Iris instance
+    - prove that you can allocate the initial state interpretation for some [x: X]
+    - prove a weakest precondition for all choices of [x: X]
+
+  Then you obtain the result of [wp_adequacy] for your choice of [X] and [I]. *)
+Local Existing Instance invGS_wsat.
+Lemma SAT_wp_adequacy {Λ} `{!invGpreS Σ} (X: Type) (I: X → irisGS Λ Σ) κs σ1 σ2 ns nt n s e es φ k P:
+  (* allocate the initial state interpretation *)
+  (∀ (iv: invGS Σ) (F: iProp Σ), SAT Alloc F [view ⊤; supply 0] True →
+   ∃ (x: X),
+    let i: irisGS Λ Σ := I x in
+    let inv: invGS Σ := iris_invGS in (* we ensure that all inferences of [invGS] point to this instance *)
+    SAT Alloc F [view ⊤; supply n] (state_interp σ1 nt κs ns ∗ P x)) →
+  (* prove the weakest precondition for all choices of [X] *)
+  (∀ x, let i: irisGS Λ Σ := I x in P x ⊢ WP e @ s; ⊤ {{ v, ⌜φ v⌝%I }}) →
+  (* then any k-step execution is safe: *)
+  language.nsteps k ([e], σ1) κs (es, σ2) →
+  (∀ v es', es = language.of_val v :: es' → φ v) ∧
+  (∀ e, s = NotStuck → e ∈ es → not_stuck e σ2).
+Proof.
+  intros Halloc Hwp Hsteps.
+  pose proof (SAT_intro (Σ := Σ)) as Hsat.
+  eapply SAT_alloc_fancy_updates in Hsat as [Hi Hsat].
+  eapply (Halloc Hi True%I) in Hsat as (x & Hsat); eauto; simpl in *.
+  eapply SAT_mono in Hsat; last first.
+  { iIntros "SI". iPoseProof (Hwp x) as "Hwp". iCombine "SI Hwp" as "Hx". iExact "Hx". }
+  eapply (@wp_adequacy _ Σ (I x)), Hsteps.
+  eapply SAT_mono, Hsat.
+  { iIntros "([$ P] & Hwp)". by iApply "Hwp". }
+Qed.
+
+
+(* Definition of adequacy *)
+Record adequate {Λ} (s : stuckness) (e1 : expr Λ) (σ1 : state Λ)
+    (φ : val Λ → state Λ → Prop) := {
+  adequate_result t2 σ2 v2 :
+   rtc erased_step ([e1], σ1) (of_val v2 :: t2, σ2) → φ v2 σ2;
+  adequate_not_stuck t2 σ2 e2 :
+   s = NotStuck →
+   rtc erased_step ([e1], σ1) (t2, σ2) →
+   e2 ∈ t2 → not_stuck e2 σ2
+}.
+
+Lemma adequate_alt {Λ} s e1 σ1 (φ : val Λ → state Λ → Prop) :
+  adequate s e1 σ1 φ ↔ ∀ t2 σ2,
+    rtc erased_step ([e1], σ1) (t2, σ2) →
+      (∀ v2 t2', t2 = of_val v2 :: t2' → φ v2 σ2) ∧
+      (∀ e2, s = NotStuck → e2 ∈ t2 → not_stuck e2 σ2).
+Proof.
+  split.
+  - intros []; naive_solver.
+  - constructor; naive_solver.
+Qed.
+
+Lemma SAT_wp_adequate {Λ} `{!invGpreS Σ} (X: Type) (I: X → irisGS Λ Σ) σ1 ns nt n s e φ P:
+  (* allocate the initial state interpretation *)
+  (∀ (iv: invGS Σ) (F: iProp Σ) κs, SAT Alloc F [view ⊤; supply 0] True →
+   ∃ (x: X),
+    let i: irisGS Λ Σ := I x in
+    let inv: invGS Σ := iris_invGS in (* we ensure that all inferences of [invGS] point to this instance *)
+    SAT Alloc F [view ⊤; supply n] (state_interp σ1 nt κs ns ∗ P x)) →
+  (* prove the weakest precondition for all choices of [X] *)
+  (∀ x, let i: irisGS Λ Σ := I x in P x ⊢ WP e @ s; ⊤ {{ v, ⌜φ v⌝%I }}) →
+  adequate s e σ1 (λ v _, φ v).
+Proof.
+  intros Halloc Hwp.
+  apply adequate_alt; intros t2 σ2' [k [κs Hsteps]]%erased_steps_nsteps.
+  eapply SAT_wp_adequacy; eauto.
+Qed.
+
 
 
 (* -------------------------------------------------------------------------- *)
